

不定积分竞赛题参考答案

$$1. \int \frac{e^{\sqrt{x}} + \sin(2\sqrt{x}+1)}{2\sqrt{x}} dx = \int [e^{\sqrt{x}} + \sin(2\sqrt{x}+1)] d\sqrt{x} = \int e^t + \sin(2t+1) dt$$

$$= e^t - \frac{1}{2} \cos(2t+1) + C = e^{\sqrt{x}} - \frac{1}{2} \cos(2\sqrt{x}+1) + C$$

$$2. \int \frac{1 + \sin^2 x}{1 - \cos 2x} dx$$

$$= \int \frac{1 + \sin^2 x}{1 - (1 - 2\sin^2 x)} dx = \int \frac{1 + \sin^2 x}{2\sin^2 x} dx = \int \left(\frac{1}{2\sin^2 x} + \frac{1}{2} \right) dx = -\frac{1}{2} \cot x + \frac{1}{2} x + C$$

$$3. \int \frac{1 + 2\cos x}{\sin^2 x} dx$$

$$= \int \left(\frac{1}{\sin^2 x} + \frac{2\cos x}{\sin^2 x} \right) dx = -\cot x + 2 \int \frac{1}{\sin^2 x} d\sin x = -\cot x - \frac{2}{\sin x} + C$$

$$4. \int \frac{3x + 2\arcsin x}{\sqrt{1-x^2}} dx$$

$$= \int \left(\frac{3x}{\sqrt{1-x^2}} + \frac{2\arcsin x}{\sqrt{1-x^2}} \right) dx = -\frac{3}{2} \int \frac{1}{\sqrt{1-x^2}} d(1-x^2) + 2 \int \arcsin x d\arcsin x$$

$$= -3\sqrt{1-x^2} + \arcsin^2 x + C$$

$$5. \int \frac{x \arctan x^2 - 3x^3 + 2x}{1+x^4} dx$$

$$= \frac{1}{2} \int \frac{\arctan x^2 - 3x^2 + 2}{1+x^4} dx^2 = \frac{1}{2} \int \frac{\arctan t - 3t + 2}{1+t^2} dt = \frac{1}{2} \int \left(\frac{\arctan t}{1+t^2} - \frac{3t}{1+t^2} + \frac{2}{1+t^2} \right) dt$$

$$= \frac{1}{2} \left[\int \arctan t d\arctan t - \frac{3}{2} \int \frac{1}{1+t^2} d(1+t^2) \right] + 2 \arctan t$$

$$= \frac{1}{4} \arctan^2 t - \frac{3}{4} \ln(1+t^2) + 2 \arctan t + C = \frac{1}{4} \arctan^2 x^2 - \frac{3}{4} \ln(1+x^4) + 2 \arctan x^2 + C$$

$$6. \text{ 令 } \sqrt{x+3} = t$$

$$\int \frac{3dx}{(x+2)\sqrt{x+3}} = 3 \int \frac{2tdt}{(t^2-1)t} = 3 \int \frac{2}{t^2-1} dt = 3 \int \left[\frac{1}{t-1} - \frac{1}{t+1} \right] dt = 3 \ln \left| \frac{t-1}{t+1} \right| + C$$

$$= 3 \ln \left| \frac{\sqrt{x+3}-1}{\sqrt{x+3}+1} \right| + C$$

$$\begin{aligned} 7. \int \frac{\sin^2 x \cos x}{1+4\sin^2 x} dx &= \int \frac{\sin^2 x}{1+4\sin^2 x} d \sin x = \frac{1}{4} \int \frac{4\sin^2 x}{1+4\sin^2 x} d \sin x \\ &= \frac{1}{4} \int \frac{1+4\sin^2 x-1}{1+4\sin^2 x} d \sin x = \frac{1}{4} \int \frac{1+4\sin^2 x-1}{1+4\sin^2 x} d \sin x = \frac{1}{4} \int 1 - \frac{1}{1+4\sin^2 x} d \sin x \\ &= \frac{1}{4} \sin x - \frac{1}{8} \arctan(2 \sin x) + C. \end{aligned}$$

$$8. \int \frac{x^3}{\sqrt{4-x^2}} dx = \frac{1}{2} \int \frac{x^2}{\sqrt{4-x^2}} dx^2 = \frac{1}{2} \int \frac{t}{\sqrt{4-t}} dt$$

$$\text{令 } \sqrt{4-t} = u$$

$$\text{所以 } \int \frac{x^3}{\sqrt{4-x^2}} dx$$

=

$$\frac{1}{2} \int \frac{t}{\sqrt{4-t}} dt = \frac{1}{2} \int \frac{4-u^2}{u} (-2u du) = \int (u^2-4) du = \frac{u^3}{3} - 4u + C = \frac{1}{3} (4-x^2)^{\frac{3}{2}} - 4\sqrt{4-x^2} + C$$

或者：令 $x = 2 \sin t$

$$\begin{aligned} \int \frac{x^3}{\sqrt{4-x^2}} dx &= \int \frac{8\sin^3 t}{2\cos t} \cdot 2\cos t dt = 8 \int \sin^3 t dt = -8 \int (1-\cos^2 t) d \cos t \\ &= \frac{8}{3} \cos^3 t - 8 \cos t + C = \frac{8}{3} \left(\frac{\sqrt{4-x^2}}{2} \right)^3 - 8 \cdot \frac{\sqrt{4-x^2}}{2} + C = \frac{1}{3} \left(\sqrt{4-x^2} \right)^{\frac{3}{2}} - 4\sqrt{4-x^2} + C \end{aligned}$$

$$9. \int \frac{\ln \cos x}{\cos^2 x} dx$$

$$= \int \ln \cos x d \tan x = \ln \cos x \cdot \tan x - \int \tan x d \ln \cos x = \ln \cos x \cdot \tan x - \int \tan x \frac{-\sin x}{\cos x} dx$$

$$= \ln \cos x \cdot \tan x + \int \tan^2 x dx = \ln \cos x \cdot \tan x + \int (\sec^2 x - 1) dx$$

$$= \ln \cos x \cdot \tan x + \tan x - x + C$$

$$10. \int \frac{1+x+2\cos x}{\sin^2 x} dx$$

$$\begin{aligned}
&= \int \left(\frac{1}{\sin^2 x} + \frac{x}{\sin^2 x} + \frac{2 \cos x}{\sin^2 x} \right) dx = -\cot x - \int x d \cot x + 2 \int \frac{1}{\sin^2 x} d \sin x \\
&= -\cot x - [x \cot x - \int \cot x dx] - \frac{2}{\sin x} = -\cot x - x \cot x + \ln |\sin x| - \frac{2}{\sin x} + C
\end{aligned}$$

$$11. \int (x+1) \log_2 x dx$$

$$\begin{aligned}
&= \int \log_2 x d \left(\frac{x^2}{2} + x \right) = \left(\frac{x^2}{2} + x \right) \log_2 x - \int \left(\frac{x^2}{2} + x \right) d \log_2 x \\
&= \left(\frac{x^2}{2} + x \right) \log_2 x - \int \left(\frac{x^2}{2} + x \right) \frac{1}{x \ln 2} dx \\
&= \left(\frac{x^2}{2} + x \right) \log_2 x - \frac{1}{\ln 2} \int \left(\frac{x}{2} + 1 \right) dx = \left(\frac{x^2}{2} + x \right) \log_2 x - \frac{1}{\ln 2} \left(\frac{x^2}{4} + x \right) + C
\end{aligned}$$

$$12. \int (3x+1) \sin 2x dx$$

$$\begin{aligned}
&= \int (3x+1) d \left(-\frac{1}{2} \cos 2x \right) = -\frac{1}{2} (3x+1) \cos 2x + \frac{1}{2} \int \cos 2x d(3x+1) \\
&= -\frac{1}{2} (3x+1) \cos 2x + \frac{3}{2} \int \cos 2x dx = -\frac{1}{2} (3x+1) \cos 2x + \frac{3}{4} \sin 2x + C
\end{aligned}$$

$$13. \int x^3 \arctan x^2 dx$$

$$\begin{aligned}
&= \frac{1}{2} \int x^2 \arctan x^2 dx^2 = \frac{1}{2} \int t \arctan t dt = \frac{1}{4} \int \arctan t dt^2 = \frac{1}{4} t^2 \arctan t - \frac{1}{4} \int t^2 d \arctan t \\
&= \frac{1}{4} t^2 \arctan t - \frac{1}{4} \int \frac{t^2}{1+t^2} dt = \frac{1}{4} t^2 \arctan t - \frac{1}{4} \int \frac{1+t^2-1}{1+t^2} dt \\
&= \frac{1}{4} t^2 \arctan t - \frac{1}{4} t + \frac{1}{4} \arctan t + C = \frac{1}{4} x^4 \arctan x^2 - \frac{1}{4} x^2 + \frac{1}{4} \arctan x^2 + C
\end{aligned}$$

$$14. \int e^x \arcsin(3e^x - 2) dx$$

$$\begin{aligned}
&= \frac{1}{3} \int \arcsin(3e^x - 2) d(3e^x - 2) = \frac{1}{3} \int \arcsin t dt = \frac{1}{3} t \arcsin t - \frac{1}{3} \int t d \arcsin t \\
&= \frac{1}{3} t \arcsin t - \frac{1}{3} \int \frac{t}{\sqrt{1-t^2}} dt = \frac{1}{3} t \arcsin t + \frac{1}{6} \int \frac{1}{\sqrt{1-t^2}} d(1-t^2) \\
&= \frac{1}{3} t \arcsin t + \frac{1}{3} \sqrt{1-t^2} + C = \frac{1}{3} (3e^x - 2) \arcsin(3e^x - 2) + \frac{1}{3} \sqrt{1-(3e^x - 2)^2} + C
\end{aligned}$$

$$15. \int \frac{xe^x}{(1+e^x)^2} dx$$

$$= \int \frac{x}{(1+e^x)^2} d(1+e^x) = \int x d\left(-\frac{1}{1+e^x}\right) = -\frac{x}{1+e^x} + \int \frac{1}{1+e^x} dx$$

$$= -\frac{x}{1+e^x} + \int \frac{1+e^x - e^x}{1+e^x} dx = -\frac{x}{1+e^x} + x - \int \frac{1}{1+e^x} d(1+e^x) = -\frac{x}{1+e^x} + x - \ln(1+e^x) + C$$

$$16. \int e^{\sqrt[3]{4x+1}} dx$$

$$\text{令 } \sqrt[3]{4x+1} = t$$

$$\int e^{\sqrt[3]{4x+1}} dx = \frac{3}{4} \int e^t t^2 dt = \frac{3}{4} \int t^2 de^t = \frac{3}{4} t^2 e^t - \frac{3}{4} \int e^t dt^2 = \frac{3}{4} t^2 e^t - \frac{3}{2} \int e^t t dt$$

$$= \frac{3}{4} t^2 e^t - \frac{3}{2} \int t de^t = \frac{3}{4} t^2 e^t - \frac{3}{2} (te^t - \int e^t dt) = \frac{3}{4} t^2 e^t - \frac{3}{2} te^t + \frac{3}{2} e^t + C$$

$$= \frac{3}{4} (4x+1)^{\frac{2}{3}} e^{\sqrt[3]{4x+1}} - \frac{3}{2} \sqrt[3]{4x+1} e^{\sqrt[3]{4x+1}} + \frac{3}{2} e^{\sqrt[3]{4x+1}} + C$$

$$17. \int \frac{x+1}{x^2-2x+5} dx$$

$$= \frac{1}{2} \int \frac{2x+2}{x^2-2x+5} dx = \frac{1}{2} \int \frac{2x-2+4}{x^2-2x+5} dx = \frac{1}{2} \int \frac{2x-2}{x^2-2x+5} dx + 2 \int \frac{1}{x^2-2x+5} dx$$

$$= \frac{1}{2} \int \frac{1}{x^2-2x+5} d(x^2-2x+5) + 2 \int \frac{1}{4+(x-1)^2} dx$$

$$= \frac{1}{2} \ln|x^2-2x+5| + \int \frac{1}{1+(\frac{x-1}{2})^2} d\frac{x-1}{2} = \frac{1}{2} \ln|x^2-2x+5| + \arctan \frac{x-1}{2} + C$$

$$18. \int \frac{x^2+5x+2}{x^2+4} dx = \int \frac{(x^2+4)+(5x-2)}{x^2+4} dx = x + 5 \int \frac{x}{x^2+4} dx - 2 \int \frac{1}{x^2+4} dx$$

$$= x + \frac{5}{2} \int \frac{1}{x^2+4} d(x^2+4) - \int \frac{1}{1+(\frac{x}{2})^2} d\frac{x}{2} = x + \frac{5}{2} \ln(x^2+4) - \arctan \frac{x}{2} + C$$

$$19. \int x e^{\sqrt{1-x^2}} dx = -\frac{1}{2} \int e^{\sqrt{1-x^2}} d(1-x^2) = -\frac{1}{2} \int e^{\sqrt{t}} dt$$

$$\text{令 } \sqrt{t} = u$$

$$\begin{aligned}\int x e^{\sqrt{1-x^2}} dx &= -\frac{1}{2} \int e^{\sqrt{t}} dt = -\int u e^u du \\ &= -\int u d e^u = -u e^u + e^u + C = -\sqrt{1-x^2} e^{\sqrt{1-x^2}} + e^{\sqrt{1-x^2}} + C\end{aligned}$$

20. 已知 $\int e^x f(x) dx = x e^x + C$, 求 $\int x f'(2x) dx$

$$e^x f(x) = e^x + x e^x, \therefore f(x) = 1 + x$$

$$\begin{aligned}\text{所以 } \int x f'(2x) dx &= \frac{1}{2} \int x f'(2x) d2x = \frac{1}{2} \int x df(2x) = \frac{1}{2} x f(2x) - \frac{1}{2} \int f(2x) dx \\ &= \frac{1}{2} x(1+2x) - \frac{1}{2} \int (1+2x) dx = \frac{1}{2} (x+2x^2) - \frac{1}{2} (x+x^2) + C = \frac{1}{2} x^2 + C\end{aligned}$$